DRAFT: A simpler kpoly.

src/Verse/CryptoLib/Karatsuba.v
@@ -2,34 +2,56 @@
 
 We begin with a different representation of polynomials which is much
 more convenient to work with when it comes to karatsuba's algorithm.
+We start with defining a complete binary tree of depth n.
+
 The type kpoly A n captures polynomials of degree 2ⁿ -1 with
 coefficients over A.
 
  *)
 
-Inductive kpoly (A : Type) : nat -> Type :=
-| kzero  : forall n , kpoly A n
-| kconst : A -> kpoly A 0
-| ksplit : forall n, kpoly A n -> kpoly A n -> kpoly A (S n).
 
 
-Arguments kzero {A n}.
-Arguments kconst {A}.
-Arguments ksplit [A n].
+Inductive tree (A : Type) : nat -> Type :=
+| leaf : A -> tree A 0
+| node : forall n, tree A n -> tree A n -> tree A (S n).
 
+
+Arguments leaf {A}.
+Arguments node [A n].
+(* If a coefficient is None, then it is zero *)
+Definition kpoly A n := tree (option A) n.
+
+Fixpoint kzero (A : Type) (n : nat) :=
+  match n with
+  | 0 => leaf (@None A)
+  | S m => let kn := kzero A m
+          in node kn kn
+  end.
+
+Require Import List.
 Require Import Verse.CryptoLib.Polynomials.
 Require Import Arith.
-Require List.
-Import List.ListNotations.
 
+Import ListNotations.
 (** The meaning of kpoly in terms of actual polynomials *)
 
 Fixpoint denote {A n} (kp : kpoly A n) : poly A :=
   match kp with
-  | kzero => []
-  | kconst x => [(x,0)]
-  | ksplit kp1 kp2 => Polynomials.add (denote kp1) (xpownTimes (2^n) (denote kp2))
+  | leaf (Some coef) => [ (coef,0) ]
+  | leaf None        => []
+  | node kp1 kp2  => Polynomials.add (denote kp1) (xpownTimes (2^n) (denote kp2))
   end.
+
+
+Definition up {n} {A : Type}(kp : kpoly A n) : kpoly A (S n) :=
+  node kp (kzero A n).
+
+Definition xPow2Pow n {A : Type}(kp : kpoly A n) : kpoly A (S n) :=
+  node (kzero A n) kp.
+
+Require Import Arith.
+Require List.
+Import List.ListNotations.
 
 Section Evaluation.
 
@@ -37,30 +59,82 @@ Section Evaluation.
 
   Fixpoint eval {n} (eta : SR)(kp : kpoly SR n) : SR :=
     match kp with
-    | kzero => semi_ring_zero
-    | kconst x => x
-    | ksplit kp1 kp2 => (eval eta kp1 + eta^(2^n) * eval eta kp2)%ring
+    | leaf None =>  0%ring
+    | leaf (Some x)  => x
+    | node  kp1 kp2 => (eval eta kp1 + eta^(2^n) * eval eta kp2)%ring
     end.
 
 End Evaluation.
 
+Ltac crush_kpoly := repeat (Polynomials.crush_poly;
+                            match goal with
+                            | [ coef : option _ |- _ ] => destruct coef
+                            | [ n : nat |- _ ] => try (ring_simplify (2^n + (2^n + 0)))
+                            | _ => idtac
+                            end).
 
+Ltac induct_on kp :=
+  induction kp as [coef | kp1 kp2 iHkp]; crush_kpoly.
 Section Correctness.
 
   Context {eta : nat}.
 
   Lemma denote_spec : forall n (kp : kpoly nat n), eval eta kp = Polynomials.eval eta (denote kp).
     intros.
-    induction kp; simpl; trivial;
-    specialise_to_nat.
-    ring.
-    rewrite power_lemma;
-    simpl; rewrite <- add_spec.
-    rewrite xpownTimes_eval.
-    repeat(rewrite Nat.pow_add_r).
-    rewrite <- IHkp1.
-    rewrite <- IHkp2.
-    trivial.
+    induct_on kp.
   Qed.
 
+  Lemma kzero_spec : forall n, eval eta (kzero nat n) = 0.
+    intro n.
+    induction n; crush_kpoly.
+    rewrite IHn; crush_kpoly.
+  Qed.
+
+  Lemma up_spec : forall n  (kp : kpoly nat n), eval eta (up kp) = eval eta kp.
+    intros n.
+    induction n.
+    intro kp. destruct kp.
+    - destruct o; simpl; specialise_to_nat; ring.
+    - unfold up. simpl. rewrite kzero_spec.
+      ring_simplify (2^n + (2^n + 0)); specialise_nat_ring.
+    - intro kp; destruct kp. unfold up; destruct o; simpl; specialise_to_nat; ring.
+      unfold up; simpl; repeat (specialise_to_nat). ring_simplify (2^n0 + (2^n0 + 0)).
+
+  Lemma constCoef_spec : forall kp : kpoly nat 0, eval eta kp = constCoef kp;
+    intro kp.
+    inversion kp.
+
+  Lemma add_spec :  forall n (kp1 kp2 : kpoly nat n),
+      eval eta (add kp1 kp2)
+      = eval eta kp1 + eval eta kp2.
+    intros n kp1.
+    induction kp1.
+    - simpl; trivial.
+    - simpl; intro kp2. inversion kp2.
+      simpl.
+Polynomials.eval eta
+                    (Polynomials.add (denote kp1) (denote kp2)).
+    intros. induction kp1.
+    induction kp2; simpl; trivial; specialise_to_nat.
+    - ring.
+    - ring_simplify (2^n + 0).
 End Correctness.
+
+Require Import Verse.CryptoLib.Polynomials.
+Section Arithmetic.
+  Context {SR : Type}`{Semi_Ring SR}.
+
+  Fixpoint constCoef {n}(kp : kpoly SR n) : SR :=
+    match kp with
+    | kzero    => 0%ring
+    | kconst a => a
+    | ksplit k1 _ => constCoef k1
+    end.
+
+  Fixpoint add {n} (kpA : kpoly SR n) : kpoly SR n -> kpoly SR n :=
+    match kpA with
+    | kzero => fun kpB => kpB
+    | kconst a => fun kb => kconst (a + constCoef kb)%ring
+    | ksplit kA1 kA2 => fun kB => let (kB1 , kB2) := kChildren kB in
+                              ksplit (add kA1 kB1) (add kA2 kB2)
+    end.
